Reworked the definition of R to be more reminiscent of RC and RV in the paper by Ahmed

src/Language/PlutusIR/Semantics/SemanticEquivalence/Def.v
@@ -54,6 +54,150 @@ Equations? R (k : nat ) (T : Ty) (t1 t2 : Term) : Prop by wf k :=
 Proof. all: try solve [eapply e; eauto]. Qed.
 *)
 
+(* Relational interpretations of values *)
+Section RV.
+
+  Context (RC : forall (k j : nat), Ty -> Term -> Term -> j < k -> Prop).
+
+  Definition RV_TyVar (k : nat) (a : tyname) (v1 v2 : Term) : Prop :=
+    False.
+
+  Definition RV_TyLam (k : nat) (bX : binderTyname) (K : Kind) (T : Ty) (v1 v2 : Term) : Prop :=
+    False.
+
+  Definition RV_TyApp (k : nat) (T1 T2 : Ty) (v1 v2 : Term) : Prop :=
+    False.
+
+  Definition RV_TyBuiltin (k : nat) (st : @some typeIn) (v1 v2 : Term) : Prop :=
+    forall sv sv',
+      (* Determine the shape of v1 and v2 *)
+      v1 = Constant sv ->
+      v2 = Constant sv' ->
+      (* Syntactic equality *)
+      v1 = v2.
+
+  Definition RV_TyFun (k : nat) (T1 T2 : Ty) (v1 v2 : Term) : Prop :=
+    forall x T e x' T' e',
+      (* Determine the shape of v1 and v2 *)
+      v1 = LamAbs x T e ->
+      v2 = LamAbs x' T' e' ->
+      (* Extensional equivalence *)
+      forall j (Hlt_j : j < k) v v' e_subst e'_subst,
+        RC k j T1 v v' Hlt_j ->
+        substitute x v e e_subst ->
+        substitute x' v' e' e'_subst ->
+        RC k j T2 e_subst e'_subst Hlt_j.
+
+
+  Definition RV_TyIFix (k : nat) (F T : Ty) (v1 v2 : Term) : Prop :=
+    forall v v',
+      (* Determine the shape of v1 and v2 *)
+      v1 = IWrap F T v ->
+      v2 = IWrap F T v' ->
+      (* Uwrap *)
+      forall j (Hlt_j : j < k) K,
+        emptyContext |-* T : K ->
+        RC k j (beta_reduce (unwrapIFix F K T)) v v' Hlt_j.
+
+  Definition RV_TyForall (k : nat) (bX : binderTyname) (K : Kind) (T : Ty) (v1 v2 : Term) : Prop :=
+    forall e e',
+      (* Determine the shape of v1 and v2 *)
+      v1 = TyAbs bX K e ->
+      v2 = TyAbs bX K e' ->
+      (* Instantiational equivalence *)
+      forall j (Hlt_j : j < k) T2,
+        RC k j (beta_reduce (substituteT bX T2 T)) e e' Hlt_j.
+
+  Definition RV (k : nat) (T : Ty) (v1 v2 : Term) : Prop :=
+    match T with
+    | Ty_Var a => RV_TyVar k a v1 v2
+    | Ty_Lam bX K T => RV_TyLam k bX K T v1 v2
+    | Ty_App T1 T2 => RV_TyApp k T1 T2 v1 v2
+    | Ty_Builtin st => RV_TyBuiltin k st v1 v2
+    | Ty_Fun T1 T2 => RV_TyFun k T1 T2 v1 v2
+    | Ty_IFix F T => RV_TyIFix k F T v1 v2
+    | Ty_Forall bX K T => RV_TyForall k bX K T v1 v2
+    end.
+End RV.
+
+
+(** RV = Relational interpretation for values, RC = Relation interpretation for computations *)
+Equations? RC (k : nat) (T : Ty) (e e' : Term) : Prop by wf k :=
+  RC k T e e' =>
+    (* RC *)
+    emptyContext |-+ e : T /\
+    emptyContext |-+ e' : T /\
+    forall j (Hlt_j : j < k) e_f,
+      e =[j]=> e_f ->
+      exists e'_f j', e' =[j']=> e'_f /\
+      
+      (* RV *)
+      match T with
+
+        (* RV for type variable *)
+        | Ty_Var a =>  
+            False
+
+        (* RV for type lambda *)
+        | Ty_Lam bX K T =>
+            False
+
+        (* RV for type application *)
+        | Ty_App T1 T2 => 
+            False
+
+        (* RV for built-in types *)
+        | Ty_Builtin st => 
+            forall v v' sv sv',
+              (* Determine the shape of e_f and e'_f *)
+              e_f = v ->
+              e'_f = v' ->
+              v = Constant sv ->
+              v' = Constant sv' ->
+              (* Syntactic equality *)
+              v = v'
+
+        (* RV for function types *)
+        | Ty_Fun T1 T2 =>
+            forall x e_body x' e'_body,
+              (* Determine the shape of e_f and e'_f *)
+              e_f = LamAbs x T1 e_body ->
+              e'_f = LamAbs x' T1 e'_body ->
+              (* Extensional equivalence *)
+              forall i (Hlt_i : i < k - j) v v' e_body' e'_body',
+                RC i T1 v v' ->
+                substitute x v e_body e_body' ->
+                substitute x' v' e'_body e'_body' ->
+                RC i T2 e_body' e'_body'
+
+        (* RV for recursive types *)
+        | Ty_IFix F T =>
+            forall v v',
+              (* Determine the shape of e_f and e_f' *)
+              e_f = IWrap F T v ->
+              e'_f = IWrap F T v' ->
+              (* Uwrap *)
+              forall i (Hlt_i : i < k - j) K,
+                emptyContext |-* T : K ->
+                RC i (beta_reduce (unwrapIFix F K T)) v v'
+
+        (* RV for universal types *)
+        | Ty_Forall bX K T => 
+            forall e_body e'_body,
+              (* Determine the shape of e_f and e_f' *)
+              e_f = TyAbs bX K e_body ->
+              e'_f = TyAbs bX K e'_body ->
+              (* Instantiational equivalence *)
+              forall i (Hlt_i : i < k - j) T2,
+                RC i (beta_reduce (substituteT bX T2 T)) e_body e'_body
+      end.
+Proof. all: try (eapply e; eauto). Qed.
+      
+      
+      
+      
+
+(*
 Equations? R (k : nat ) (T : Ty) (t1 t2 : Term) : Prop by wf k :=
   R k T t1 t2 =>
     emptyContext |-+ t1 : T /\
@@ -105,6 +249,7 @@ Equations? R (k : nat ) (T : Ty) (t1 t2 : Term) : Prop by wf k :=
     | _ => False (* Ty_Lam, Ty_Lam and Ty_Var should not occur *)
     end.
 Proof. all: try solve [eapply e; eauto]. Qed.
+*)
 
 Definition possible_type (T : Ty) : Prop :=
   match T with
@@ -117,118 +262,138 @@ Definition possible_type (T : Ty) : Prop :=
 
 Definition impossible_type (T : Ty) : Prop := ~ possible_type T.
 
-Lemma R_typable_empty : forall k T t1 t2,
-    R k T t1 t2 ->
-    emptyContext |-+ t1 : T /\ emptyContext |-+ t2 : T.
-Proof. intros. destruct k, T; destruct H as [Ht1 [Ht2 _]]; auto. Qed.
+Lemma RC_typable_empty : forall k T e e',
+    RC k T e e' ->
+    emptyContext |-+ e : T /\ emptyContext |-+ e' : T.
+Proof. intros. destruct k, T; destruct H as [He [He' _]]; auto. Qed.
 
-Lemma R_typable_empty_1 : forall k T t1 t2,
-    R k T t1 t2 ->
-    emptyContext |-+ t1 : T.
-Proof. intros. destruct (R_typable_empty _ _ _ _ H). assumption. Qed.
+Lemma RC_typable_empty_1 : forall k T e e',
+    RC k T e e' ->
+    emptyContext |-+ e : T.
+Proof. intros. destruct (RC_typable_empty _ _ _ _ H). assumption. Qed.
 
-Lemma R_typable_empty_2 : forall k T t1 t2,
-    R k T t1 t2 ->
-    emptyContext |-+ t2 : T.
-Proof. intros. destruct (R_typable_empty _ _ _ _ H). assumption. Qed.
+Lemma RC_typable_empty_2 : forall k T e e',
+    RC k T e e' ->
+    emptyContext |-+ e' : T.
+Proof. intros. destruct (RC_typable_empty _ _ _ _ H). assumption. Qed.
 
-Lemma R_evaluable : forall k T t1 j1 v1 t2,
-    terminates_excl t1 j1 v1 k ->
-    possible_type T ->
-    R k T t1 t2 ->
-    exists v2 j2, j1 < k /\ t1 =[j1]=> v1 /\ t2 =[j2]=> v2.
-Proof. intros. destruct H. autorewrite with R in H1.
-  destruct T; inversion H0; destruct H1 as [_ [_ [v2 [j2 [Hev2 _]]]]]; eauto; 
-    try solve [eexists; eexists; eexists; eexists; eauto].
+Lemma RC_evaluable : forall k T e j e_f e',
+    terminates_excl e j e_f k ->
+    RC k T e e' ->
+    exists e'_f j', j < k /\ e =[j]=> e_f /\ e' =[j']=> e'_f.
+Proof. intros. destruct H. autorewrite with RC in H1.
+  destruct T; destruct H0 as [_ [_ [e'_f [j' [Hev_e' _]]]]]; eauto.
+  Unshelve. all: eauto.
 Qed.
 
-Lemma R_evaluable_1 : forall k T t1 j1 v1 t2,
-    terminates_excl t1 j1 v1 k ->
-    possible_type T ->
-    R k T t1 t2 ->
-    j1 < k /\ t1 =[j1]=> v1.
+Lemma RC_evaluable_1 : forall k T e j e_f e',
+    terminates_excl e j e_f k ->
+    RC k T e e' ->
+    j < k /\ e =[j]=> e_f.
 Proof. intros. destruct H. eauto. Qed.
 
-Lemma R_evaluable_2 : forall k T t1 j1 v1 t2,
-    terminates_excl t1 j1 v1 k ->
-    possible_type T ->
-    R k T t1 t2 ->
-    exists v2 j2, t2 =[j2]=> v2.
-Proof. intros. destruct (R_evaluable _ _ _ _ _ _ H H0 H1) as [v2 [j2 [_ [_ Hev2]]]]; eauto. Qed.
+Lemma RC_evaluable_2 : forall k T e j e_f e',
+    terminates_excl e j e_f k ->
+    RC k T e e' ->
+    exists e'_f j', e' =[j']=> e'_f.
+Proof. intros. destruct (RC_evaluable _ _ _ _ _ _ H H0) as [e'_f [j' [_ [_ Hev_e']]]]; eauto. Qed.
 
-Lemma R_syntactic_equality : forall k st t1 j1 v1 t2,
-    terminates_excl t1 j1 v1 k ->
-    R k (Ty_Builtin st) t1 t2 ->
-    exists v2 j2,
-      t2 =[j2]=> v2 /\
-      v1 = v2.
-Proof. intros. destruct H. destruct H0 as [_ [_ [v2 [j2 [Hev2 Heq]]]]]; eauto. Qed.
+Lemma RC_syntactic_equality : forall k st e j e_f e',
+    terminates_excl e j e_f k ->
+    RC k (Ty_Builtin st) e e' ->
 
-Lemma R_functional_extensionality : forall k T1 T2 t1 j1 v1 t2,
-    terminates_excl t1 j1 v1 k ->
-    R k (Ty_Fun T1 T2) t1 t2 ->
-    exists v2 j2,
-      t2 =[j2]=> v2 /\
-      (forall s1 s2 k' x1_0 x2_0 T1_0 T2_0 t1_0 t2_0 t1_0' t2_0',
-        k' < k - j1 ->
-        v1 = LamAbs x1_0 T1_0 t1_0 ->
-        v2 = LamAbs x2_0 T2_0 t2_0 ->
-        R k' T1 s1 s2 ->
-        substitute x1_0 s1 t1_0 t1_0' ->
-        substitute x2_0 s2 t2_0 t2_0' ->
-        R k' T2 t1_0' t2_0').
+    (exists e'_f j',
+      e' =[j']=> e'_f /\
+
+      forall v v' sv sv',
+        (* Determine the shape of e_f and e'_f *)
+        e_f = v ->
+        e'_f = v' ->
+        v = Constant sv ->
+        v' = Constant sv' ->
+        (* Syntactic equality *)
+        v = v').
+Proof. intros. destruct H. destruct H0 as [_ [_ [e'_f [j' [Hev_e' Heq]]]]]; eauto. Qed.
+
+Lemma RC_functional_extensionality : forall k T1 T2 e j e_f e',
+    terminates_excl e j e_f k ->
+    RC k (Ty_Fun T1 T2) e e' ->
+
+    exists e'_f j',
+      e' =[j']=> e'_f /\
+
+      (forall x e_body x' e'_body,
+        (* Determine the shape of e_f and e'_f *)
+        e_f = LamAbs x T1 e_body ->
+        e'_f = LamAbs x' T1 e'_body ->
+        (* Extensional equivalence *)
+        forall i (Hlt_i : i < k - j) v v' e_body' e'_body',
+          RC i T1 v v' ->
+          substitute x v e_body e_body' ->
+          substitute x' v' e'_body e'_body' ->
+          RC i T2 e_body' e'_body').
 Proof. 
-  intros k T1 T2 t1 j1 v1 t2 Hterm R. 
+  intros k T1 T2 t1 j1 v1 t2 Hterm RC. 
   destruct Hterm.
-  autorewrite with R in R.
-  destruct R as [_ [_ [v2 [j2 [Hev_t2 Hfe]]]]]; eauto.
+  autorewrite with RC in RC.
+  destruct RC as [_ [_ [e'_f [j' [Hev_e' Hfe]]]]]; eauto.
 Qed.
 
-Lemma R_unwrap : forall k F T t1 j1 v1 t2,
-    terminates_excl t1 j1 v1 k ->
-    R k (Ty_IFix F T) t1 t2 ->
-    exists v2 j2,
-      t2 =[j2]=> v2 /\
-      (forall K k',
-        k' < k - j1 ->
-        emptyContext |-* T : K ->
-        R k' (beta_reduce (unwrapIFix F K T)) v1 v2).
+Lemma RC_unwrap : forall k F T e j e_f e',
+    terminates_excl e j e_f k ->
+    RC k (Ty_IFix F T) e e' ->
+
+    exists e'_f j',
+      e' =[j']=> e'_f /\
+
+      (forall v v',
+        (* Determine the shape of e_f and e_f' *)
+        e_f = IWrap F T v ->
+        e'_f = IWrap F T v' ->
+        (* Uwrap *)
+        forall i (Hlt_i : i < k - j) K,
+          emptyContext |-* T : K ->
+          RC i (beta_reduce (unwrapIFix F K T)) v v').
 Proof.
-  intros k F T t1 j1 v1 t2 Hterm R.
+  intros k F T t1 j1 v1 t2 Hterm RC.
   destruct Hterm. 
-  autorewrite with R in R.
-  destruct R as [_ [_ [v2 [j2 [Hev_t2 Hunwrap]]]]]; eauto.
+  autorewrite with RC in RC.
+  destruct RC as [_ [_ [e'_f [j' [Hev_e' Hunwrap]]]]]; eauto.
 Qed.
 
-Lemma R_instantiational_extensionality : forall k X K T t1 j1 v1 t2,
-    terminates_excl t1 j1 v1 k ->
-    R k (Ty_Forall X K T) t1 t2 ->
-    exists v2 j2,
-      t2 =[j2]=> v2 /\
-      (forall t0_1 t0_2 T' k',
-        k' < k - j1 ->
-        v1 = TyAbs X K t0_1 ->
-        v2 = TyAbs X K t0_2 ->
-        emptyContext |-* T' : K ->
-        R k' (beta_reduce (substituteT X T' T)) v1 v2).
+Lemma RC_instantiational_extensionality : forall k bX K T e j e_f e',
+    terminates_excl e j e_f k ->
+    RC k (Ty_Forall bX K T) e e' ->
+
+    exists e'_f j',
+      e' =[j']=> e'_f /\
+
+      (forall e_body e'_body,
+        (* Determine the shape of e_f and e_f' *)
+        e_f = TyAbs bX K e_body ->
+        e'_f = TyAbs bX K e'_body ->
+        (* Instantiational equivalence *)
+        forall i (Hlt_i : i < k - j) T2,
+          RC i (beta_reduce (substituteT bX T2 T)) e_body e'_body).
 Proof.
-  intros k X K T t1 j1 v1 t2 Hterm R. 
+  intros k X K T t1 j1 v1 t2 Hterm RC. 
   destruct Hterm.
-  autorewrite with R in R.
-  destruct R as [_ [_ [v2 [j2 [Hev_t2 Hie]]]]]; eauto.
+  autorewrite with RC in RC.
+  destruct RC as [_ [_ [e'_f [j' [Hev_e' Hie]]]]]; eauto.
 Qed.
 
 
-Lemma R_impossible_type : forall k t1 t2,
-    (forall a, ~(R k (Ty_Var a) t1 t2)) /\
-    (forall bX K T, ~(R k (Ty_Lam bX K T) t1 t2)) /\
-    (forall T1 T2, ~(R k (Ty_App T1 T2) t1 t2)).
-Proof. intros. split; try split; try solve [intros; intro Hcon; destruct k; destruct Hcon as [_ [_ Hfls]]; eauto]. Qed.
+Lemma RC_impossible_type : forall k e j e_f e',
+    terminates_excl e j e_f k ->
 
-Lemma R_nontermination : forall k T t1 t2,
-    ~(exists j1 v1, terminates_excl t1 j1 v1 k) ->
-    possible_type T ->
-    emptyContext |-+ t1 : T ->
-    emptyContext |-+ t2 : T ->
-    R k T t1 t2.
+    (forall a, ~(RC k (Ty_Var a) e e')) /\
+    (forall bX K T, ~(RC k (Ty_Lam bX K T) e e')) /\
+    (forall T1 T2, ~(RC k (Ty_App T1 T2) e e')).
+Proof. intros. destruct H. split; try split; try solve [intros; intro Hcon; destruct Hcon as [_ [_ [_ [_ [_ Hfls]]]]]; eauto]. Qed.
+
+Lemma RC_nontermination : forall k T e e',
+    ~(exists e_f j, terminates_excl e j e_f k) ->
+    emptyContext |-+ e : T ->
+    emptyContext |-+ e' : T ->
+    RC k T e e'.
 Proof. intros. unfold terminates_excl in H. destruct T; try solve [split; auto; split; auto; intros; exfalso; apply H; eauto]. Qed.
