src/Language/PlutusIR/Semantics/SemanticEquivalence/ReductionInvariance.v
@@ -21,7 +21,7 @@ Proof.
     + assumption.
 Qed.
 
-Lemma e : forall j k i,
+Lemma helper : forall j k i,
     0 < k ->
     j < k - 0 ->
     j < k - i.
@@ -31,203 +31,246 @@ Proof. Admitted.
 
 (** ** Evaluation of the first related term preserves [R] *)
 
-Lemma eval_preserves_R_left : forall k T t1 j1 v1 t2,
-    terminates_excl t1 j1 v1 k ->
-    R k T t1 t2 ->
-    R k T v1 t2.
+Lemma eval_preserves_R_left : forall k T e j e_f e',
+    terminates_excl e j e_f k ->
+    RC k T e e' ->
+    RC k T e_f e'.
 Proof.
-  intros k T t1 j1 v1 t2 Hterm R.
-  destruct Hterm as [Hev_t1 Hlt_j1] eqn:Hterm'.
+  intros k T e j e_f e' Hterm RC.
+  destruct Hterm as [Hev__e Hlt__j] eqn:Hterm'.
 
-  assert (emptyContext |-+ t1 : T) by eauto using R_typable_empty_1.
-  assert (emptyContext |-+ t2 : T) by eauto using R_typable_empty_2.
-  assert (emptyContext |-+ v1 : T) by eauto using preservation.
+  assert (emptyContext |-+ e : T) by eauto using RC_typable_empty_1.
+  assert (emptyContext |-+ e' : T) by eauto using RC_typable_empty_2.
+  assert (emptyContext |-+ e_f : T) by eauto using preservation.
 
-  autorewrite with R.
+  autorewrite with RC.
   destruct T.
-  - apply R_impossible_type in R. destruct R.
-  - eapply R_functional_extensionality in R as Hfe; eauto.
-    destruct Hfe as [v2 [j2 [Hev_t2 Hfe]]].
+  - (* Ty_Var *)
+    eapply RC_impossible_type in RC; eauto. destruct RC.
+
+  - (* Ty_Fun *)
+    eapply RC_functional_extensionality in RC as Hfe; eauto.
+    destruct Hfe as [e'_f [j' [Hev__e' Hfe]]].
   
     split; auto. split; auto.
-    intros v0 j0 Hlt_j0 Hev_v1.
-    exists v2, j2. split; auto.
+    intros j0 Hlt__j0 e_f0 Hev__e_f.
+    exists e'_f, j'. split; auto.
     
-    intros s1 s2 k' x1_0 x2_0 T1_0 T2_0 t1_0 t2_0 t1_0' t2_0' Hlt_k' Heq1_0 Heq2_0 R' Hsubst1_0 Hsubst2_0. 
-    apply eval_to_value in Hev_t1 as Hval_v1.
-    apply eval_value in Hval_v1.
-    unfold P_value in Hval_v1.
-    assert (v0 = v1 /\ j0 = 0) by (eapply eval__deterministic; eauto).
+    intros x e_body x' e'_body Heq1 Heq2 i Hlt__i  v v' e_body' e'_body' RC' Hsubst Hsubst'.
+
+    apply eval_to_value in Hev__e as Hval__e_f.
+    apply eval_value in Hval__e_f.
+    unfold P_value in Hval__e_f.
+    assert (e_f0 = e_f /\ j0 = 0) by (eapply eval__deterministic; eauto).
     destruct H2. subst. 
+
     eapply Hfe.
-    + eapply e; eauto.
     + reflexivity.
     + reflexivity.
+    + eapply helper; eauto.
     + eassumption.
     + assumption.
     + assumption.
+
   - (* Ty_IFix *)
-    eapply R_unwrap in R as Hunwr; eauto.
-    destruct Hunwr as [v2 [j2 [Hev_t2 Hunwr]]].
+    eapply RC_unwrap in RC as Hunwr; eauto.
+    destruct Hunwr as [e'_f [j' [Hev__e' Hunwr]]].
     
     split; auto. split; auto.
-    intros v0 j0 Hlt_j0 Hev_v1.
-    exists v2, j2. split; auto.
+    intros j0 Hlt__j0 e_f0 Hev__e_f.
+    exists e'_f, j'. split; auto.
+    
+    intros v v' Heq1 Heq2 i Hlt__i K Hkind_T2.
 
-    intros K k' Hlt_k' Hkind_T2.
-    apply eval_to_value in Hev_t1 as Hval_v1.
-    apply eval_value in Hval_v1 as Hev_v1'.
-    unfold P_value in Hev_v1'.
-    assert (v0 = v1 /\ j0 = 0) by (eapply eval__deterministic; eauto).
-    destruct H2. subst.
+    apply eval_to_value in Hev__e as Hval__e_f.
+    apply eval_value in Hval__e_f.
+    unfold P_value in Hval__e_f.
+    assert (e_f0 = e_f /\ j0 = 0) by (eapply eval__deterministic; eauto).
+    destruct H2. subst. 
+
     apply Hunwr.
-    + eapply e; eauto.
+    + reflexivity.
+    + reflexivity.
+    + eapply helper; eauto.
     + assumption.
+
   - (* Ty_Forall *)
-    eapply R_instantiational_extensionality in R as Hie; eauto.
-    destruct Hie as [v2 [j2 [Hev_t2 Hie]]].
+    eapply RC_instantiational_extensionality in RC as Hie; eauto.
+    destruct Hie as [e'_f [j' [Hev__e' Hie]]].
 
     split; auto. split; auto.
-    intros v0 j0 Hlt_j0 Hev_v1.
-    exists v2, j2. split; auto.
+    intros j0 Hlt__j0 e_f0 Hev__e_f.
+    exists e'_f, j'. split; auto.
 
-    intros t0_1 t0_2 T' k' Hlt_k' Heq1 Heq2 Hkind_T'.
-    apply eval_to_value in Hev_t1 as Hval_v1.
-    apply eval_value in Hval_v1 as Hev_v1'.
-    unfold P_value in Hev_v1'.
-    assert (v0 = v1 /\ j0 = 0) by (eapply eval__deterministic; eauto).
-    destruct H2. subst.
+    intros e_body e'_body Heq1 Heq2 Hi Hlt__i T2.
+
+    apply eval_to_value in Hev__e as Hval__e_f.
+    apply eval_value in Hval__e_f.
+    unfold P_value in Hval__e_f.
+    assert (e_f0 = e_f /\ j0 = 0) by (eapply eval__deterministic; eauto).
+    destruct H2. subst. 
+
     eapply Hie.
-    + apply e; eauto.
     + reflexivity.
     + reflexivity.
-    + assumption.
+    + apply helper; eauto.
+
   - (* Ty_Builtin *)
-    eapply R_syntactic_equality in R as Hse; eauto.
-    destruct Hse as [v2 [j2 [Hev_t2 Hse]]].
+    eapply RC_syntactic_equality in RC as Hse; eauto.
+    destruct Hse as [e'_f [j' [Hev__e' Hse]]].
     subst.
 
     split; auto. split; auto.
-    intros v0 j0 Hlt_j0 Hev_v1.
-    exists v2, j2. split; auto.
+    intros j0 Hlt__j0 e_f0 Hev__e_f.
+    exists e'_f, j'. split; auto.
 
-    apply eval_to_value in Hev_t1 as Hval_v1.
-    apply eval_value in Hval_v1 as Hev_v1'.
-    unfold P_value in Hev_v1'.
-    assert (v0 = v2 /\ j0 = 0) by (eapply eval__deterministic; eauto).
-    destruct H2. subst.
-    reflexivity.
+    intros v v' sv sv' Heq1 Heq2 Heq3 Heq4.
+
+    apply eval_to_value in Hev__e as Hval__e_f.
+    apply eval_value in Hval__e_f.
+    unfold P_value in Hval__e_f.
+    assert (e_f0 = e_f /\ j0 = 0) by (eapply eval__deterministic; eauto).
+    destruct H2. subst. 
+
+    eapply Hse; auto.
+
   - (* Ty_Lam *)
-    apply R_impossible_type in R. destruct R.
+    eapply RC_impossible_type in RC; eauto. destruct RC.
+
   - (* Ty_App *)
-    apply R_impossible_type in R. destruct R.
+    eapply RC_impossible_type in RC; eauto. destruct RC.
 Qed.
 
 (** ** Evaluation of the second related term preserves [R] *)
 
-Lemma eval_preserves_R_right : forall k T t1 j1 v1 t2 j2 v2,
-    terminates_excl t1 j1 v1 k ->
-    t2 =[j2]=> v2 ->
-    R k T t1 t2 ->
-    R k T t1 v2.
-Proof. 
-  intros k T t1 j1 v1 t2 j2 v2 Hterm Hev_t2 R.
-  destruct Hterm as [Hev_t1 Hlt_j1] eqn:Hterm'.
+(*
+Lemma eval_preserves_R_left : forall k T e j e_f e',
+    terminates_excl e j e_f k ->
+    RC k T e e' ->
+    RC k T e_f e'.
+Proof.
+  intros k T e j e_f e' Hterm RC.
+  destruct Hterm as [Hev__e Hlt__j] eqn:Hterm'.
 
-  assert (emptyContext |-+ t1 : T) by eauto using R_typable_empty_1.
-  assert (emptyContext |-+ t2 : T) by eauto using R_typable_empty_2.
-  assert (emptyContext |-+ v2 : T) by eauto using preservation.
+  assert (emptyContext |-+ e : T) by eauto using RC_typable_empty_1.
+  assert (emptyContext |-+ e' : T) by eauto using RC_typable_empty_2.
+  assert (emptyContext |-+ e_f : T) by eauto using preservation.
 
-  autorewrite with R.
+  autorewrite with RC.
   destruct T.
-  - apply R_impossible_type in R. destruct R.
-  - eapply R_functional_extensionality in R as Hfe; eauto.
-    destruct Hfe as [v2' [j2' [Hev_t2' Hfe]]].
+  - (* Ty_Var *)
+    eapply RC_impossible_type in RC; eauto. destruct RC.*)
+
+Lemma eval_preserves_R_right : forall k T e j e_f e' j' e'_f,
+    terminates_excl e j e_f k ->
+    e' =[j']=> e'_f ->
+    RC k T e e' ->
+    RC k T e e'_f.
+Proof. 
+  intros k T e j e_f e' j' e'_f Hterm Hev__e' RC.
+  destruct Hterm as [Hev__e Hlt__j] eqn:Hterm'.
+
+  assert (emptyContext |-+ e : T) by eauto using RC_typable_empty_1.
+  assert (emptyContext |-+ e' : T) by eauto using RC_typable_empty_2.
+  assert (emptyContext |-+ e'_f : T) by eauto using preservation.
+
+  autorewrite with RC.
+  destruct T.
+  - (* Ty_Var *)
+    eapply RC_impossible_type in RC; eauto. destruct RC.
+
+  - (* Ty_Fun *)
+    eapply RC_functional_extensionality in RC as Hfe; eauto.
+    destruct Hfe as [e'_f0 [j'0 [Hev__e'0 Hfe]]].
   
     split; auto. split; auto.
-    intros v1' j1' Hlt_j1' Hev_t1'.
+    intros j0 Hlt__j0 e_f0 Hev__e_f.
 
-    assert (v2' = v2 /\ j2' = j2) by (eapply eval__deterministic; eauto).
+    assert (e'_f0 = e'_f /\ j'0 = j') by (eapply eval__deterministic; eauto).
     destruct H2. subst.
-    apply eval_to_value in Hev_t2 as Hval_v2.
-    apply eval_value in Hval_v2 as Hev_v2.
-    unfold P_value in Hev_v2.
+    apply eval_to_value in Hev__e' as Hval__e'_f.
+    apply eval_value in Hval__e'_f.
+    unfold P_value in Hval__e'_f.
+    exists e'_f, 0. split; auto.
 
-    exists v2, 0. split; auto.
-
-    assert (v1' = v1 /\ j1' = j1) by (eapply eval__deterministic; eauto).
+    assert (e_f0 = e_f /\ j0 = j) by (eapply eval__deterministic; eauto).
     destruct H2. subst.
 
     apply Hfe.
+
   - (* Ty_IFix *)
-    eapply R_unwrap in R as Hunwr; eauto.
-    destruct Hunwr as [v2' [j2' [Hev_t2' Hunwr]]].
+    eapply RC_unwrap in RC as Hunwr; eauto.
+    destruct Hunwr as [e'_f0 [j'0 [Hev__e'0 Hunwr]]].
 
     split; auto. split; auto.
-    intros v1' j1' Hlt_j1' Hev_t1'.
+    intros j0 Hlt__j0 e_f0 Hev__e_f.
 
-    assert (v2' = v2 /\ j2' = j2) by (eapply eval__deterministic; eauto).
+    assert (e'_f0 = e'_f /\ j'0 = j') by (eapply eval__deterministic; eauto).
     destruct H2. subst.
-    apply eval_to_value in Hev_t2 as Hval_v2.
-    apply eval_value in Hval_v2 as Hev_v2.
-    unfold P_value in Hev_v2.
+    apply eval_to_value in Hev__e' as Hval__e'_f.
+    apply eval_value in Hval__e'_f.
+    unfold P_value in Hval__e'_f.
+    exists e'_f, 0. split; auto.
 
-    exists v2, 0. split; auto.
-
-    assert (v1' = v1 /\ j1' = j1) by (eapply eval__deterministic; eauto).
+    assert (e_f0 = e_f /\ j0 = j) by (eapply eval__deterministic; eauto).
     destruct H2. subst.
 
     apply Hunwr.
+
   - (* Ty_Forall *)
-    eapply R_instantiational_extensionality in R as Hie; eauto.
-    destruct Hie as [v2' [j2' [Hev_t2' Hie]]].
+    eapply RC_instantiational_extensionality in RC as Hie; eauto.
+    destruct Hie as [e'_f0 [j'0 [Hev__e'0 Hie]]].
 
     split; auto. split; auto.
-    intros v1' j1' Hlt_j1' Hev_t1'.
+    intros j0 Hlt__j0 e_f0 Hev__e_f.
 
-    assert (v2' = v2 /\ j2' = j2) by (eapply eval__deterministic; eauto).
+    assert (e'_f0 = e'_f /\ j'0 = j') by (eapply eval__deterministic; eauto).
     destruct H2. subst.
-    apply eval_to_value in Hev_t2 as Hval_v2.
-    apply eval_value in Hval_v2 as Hev_v2.
-    unfold P_value in Hev_v2.
+    apply eval_to_value in Hev__e' as Hval__e'_f.
+    apply eval_value in Hval__e'_f.
+    unfold P_value in Hval__e'_f.
+    exists e'_f, 0. split; auto.
 
-    exists v2, 0. split; auto.
-
-    assert (v1' = v1 /\ j1' = j1) by (eapply eval__deterministic; eauto).
+    assert (e_f0 = e_f /\ j0 = j) by (eapply eval__deterministic; eauto).
     destruct H2. subst.
 
     apply Hie.
+
   - (* Ty_Builtin *)
-    eapply R_syntactic_equality in R as Hse; eauto.
-    destruct Hse as [v2' [j2' [Hev_t2' Hse]]].
+    eapply RC_syntactic_equality in RC as Hse; eauto.
+    destruct Hse as [e'_f0 [j'0 [Hev__e'0 Hse]]].
 
     split; auto. split; auto.
-    intros v1' j1' Hlt_j1' Hev_t1'.
+    intros j0 Hlt__j0 e_f0 Hev__e_f.
 
-    assert (v2' = v2 /\ j2' = j2) by (eapply eval__deterministic; eauto).
+    assert (e'_f0 = e'_f /\ j'0 = j') by (eapply eval__deterministic; eauto).
     destruct H2. subst.
-    apply eval_to_value in Hev_t2 as Hval_v2.
-    apply eval_value in Hval_v2 as Hev_v2.
-    unfold P_value in Hev_v2.
+    apply eval_to_value in Hev__e' as Hval__e'_f.
+    apply eval_value in Hval__e'_f.
+    unfold P_value in Hval__e'_f.
+    exists e'_f, 0. split; auto.
 
-    exists v2, 0. split; auto.
+    assert (e_f0 = e_f /\ j0 = j) by (eapply eval__deterministic; eauto).
+    destruct H2. subst.
 
-    eapply eval__deterministic; eauto.
+    apply Hse.
+
   - (* Ty_Lam *)
-    apply R_impossible_type in R. destruct R.
+    eapply RC_impossible_type in RC; eauto. destruct RC.
+
   - (* Ty_App *)
-    apply R_impossible_type in R. destruct R.
+    eapply RC_impossible_type in RC; eauto. destruct RC.
 Qed.
 
 (** ** Evaluation of both related terms preserves [R] *)
 
-Lemma eval_preserves_R : forall k T t1 j1 v1 t2 j2 v2,
-    terminates_excl t1 j1 v1 k ->
-    t2 =[j2]=> v2 ->
-    R k T t1 t2 ->
-    R k T v1 v2.
+Lemma eval_preserves_R : forall k T e j e_f e' j' e'_f,
+    terminates_excl e j e_f k ->
+    e' =[j']=> e'_f ->
+    RC k T e e' ->
+    RC k T e_f e'_f.
 Proof.
-  intros k T t1 j1 v1 t2 j2 v2 Hterm1 Hev2 R.
+  intros k T e j e_f e' j' e'_f Hterm Hev RC.
   eapply eval_preserves_R_left; eauto.
   eapply eval_preserves_R_right; eauto.
 Qed.
@@ -237,34 +280,34 @@ Qed.
 
 (** ** Evaluation of the first related term preserved [R] *)
 
-Lemma eval_preserved_R_left : forall k T t1 j1 v1 t2,
-    emptyContext |-+ t1 : T ->
-    terminates_excl t1 j1 v1 k ->
-    R k T v1 t2 ->
-    R k T t1 t2.
+Lemma eval_preserved_R_left : forall k T e j e_f e',
+    emptyContext |-+ e : T ->
+    terminates_excl e j e_f k ->
+    RC k T e_f e' ->
+    RC k T e e'.
 Proof. Abort.
 
 (** ** Evaluation of the second related term preserved [R] *)
 
-Lemma eval_preserved_R_right : forall k T t1 j1 v1 t2 j2 v2,
-    emptyContext |-+ t2 : T ->
-    terminates_excl t1 j1 v1 k ->
-    t2 =[j2]=> v2 ->
-    R k T t1 v2 ->
-    R k T t1 t2.
+Lemma eval_preserved_R_right : forall k T e j e_f e' j' e'_f,
+    emptyContext |-+ e' : T ->
+    terminates_excl e j e_f k ->
+    e' =[j']=> e'_f ->
+    RC k T e e'_f ->
+    RC k T e e'.
 Proof. Abort.
 
 (** ** Evaluation of the both related terms preserved [R] *)
 
-Lemma eval_preserved_R : forall k T t1 j1 v1 t2 j2 v2,
-    emptyContext |-+ t1 : T ->
-    emptyContext |-+ t2 : T ->
-    terminates_excl t1 j1 v1 k ->
-    t2 =[j2]=> v2 ->
-    R k T v1 v2 ->
-    R k T t1 t2.
+Lemma eval_preserved_R : forall k T e j e_f e' j' e'_f,
+    emptyContext |-+ e : T ->
+    emptyContext |-+ e' : T ->
+    terminates_excl e j e_f k ->
+    e' =[j']=> e'_f ->
+    RC k T e_f e'_f ->
+    RC k T e e'.
 Proof.
-  intros k T t1 j1 v1 t2 j2 v2 Htyp_t1 Htyp_t2 Hterm1 Hev2 R.
+  intros k T e j e_f e' j' e'_f Htyp__e Htyp__e' Hterm Hev RC.
   (*
   apply eval_preserved_R_left with v1; auto.
   apply eval_preserved_R_right with v2; auto.
